specs/lib/Spec.Lib.IntSeq.fsti
@@ -3,14 +3,31 @@ module Spec.Lib.IntSeq
 open Spec.Lib.IntTypes
 
 val lseq: a:Type0 -> len:size_t -> t:Type0
-
 val create: #a:Type -> len:size_t -> init:a -> lseq a len 
 val createL: #a:Type -> l:list a{List.Tot.length l <= maxint U32} -> lseq a (List.Tot.length l)
+val index: #a:Type -> #len:size_t{len > 0} -> lseq a len -> n:size_t{n < len} -> a
+val upd: #a:Type -> #len:size_t -> lseq a len -> n:size_t{n < len /\ len > 0} -> x:a -> lseq a len
+val sub: #a:Type -> #len:size_t -> lseq a len -> start:size_t -> n:size_t{start + n <= len} -> lseq a n
+val slice: #a:Type -> #len:size_t -> lseq a len -> start:size_t -> fin:size_t{start <= fin /\ fin <= len} -> lseq a (fin - start)
+val update_sub: #a:Type -> #len:size_t -> lseq a len -> start:size_t -> n:size_t{start + n <= len} -> lseq a n -> lseq a len
+val update_slice: #a:Type -> #len:size_t -> lseq a len -> start:size_t -> fin:size_t{start <= fin /\ fin <= len} -> lseq a (fin - start) -> lseq a len
 
-val repeat: #a:Type -> n:size_t -> (a -> Tot a) -> a -> Tot (a) 
+let op_String_Access = index
+let op_String_Assignment = upd
+
+
+val repeat_range: #a:Type -> min:size_t -> max:size_t{min <= max} -> (i:size_t{i >= min /\ i < max}  -> a -> Tot a) -> a -> Tot (a) 
 val repeati: #a:Type -> n:size_t -> (i:size_t{i < n}  -> a -> Tot a) -> a -> Tot (a) 
+val repeat: #a:Type -> n:size_t -> (a -> Tot a) -> a -> Tot (a) 
+
+
+
+val fold_left_range: #a:Type -> #b:Type -> #len:size_t -> min:size_t -> max:size_t{min <= max /\ max <= len} -> (i:size_t{i >= min /\ i < max} -> a -> b -> Tot b) -> lseq a len -> b -> Tot (b) 
+val fold_lefti: #a:Type -> #b:Type -> #len:size_t -> (i:size_t{i < len} -> a -> b -> Tot b) -> lseq a len -> b -> Tot (b) 
 val fold_left: #a:Type -> #b:Type -> #len:size_t -> (a -> b -> Tot b) -> lseq a len -> b -> Tot (b) 
-val fold_lefti: #a:Type -> #b:Type -> #len:size_t -> (size_t -> a -> b -> Tot b) -> lseq a len -> b -> Tot (b) 
+
+//val fold_left_slices: #a:Type -> #b:Type -> #len:size_t -> #slice_len:size_t{len % slice_len = 0} -> (lseq a slice_len -> b -> Tot b) -> lseq a len -> b -> Tot b
+
 
 val map: #a:Type -> #b:Type -> #len:size_t -> (a -> Tot b) -> lseq a len -> lseq b len
 val for_all: #a:Type -> #len:size_t -> (a -> Tot bool) -> lseq a len -> bool
@@ -22,22 +39,16 @@ val map2: #a:Type -> #b:Type -> #c:Type -> #len:size_t -> (a -> b -> Tot c) -> l
 
 val for_all2: #a:Type -> #b:Type -> #len:size_t -> (a -> b -> Tot bool) -> lseq a len -> lseq b len -> bool
 
-val index: #a:Type -> #len:size_t{len > 0} -> lseq a len -> n:size_t{n < len} -> a
-
-val upd: #a:Type -> #len:size_t -> lseq a len -> n:size_t{n < len /\ len > 0} -> x:a -> lseq a len
-
-val sub: #a:Type -> #len:size_t -> lseq a len -> start:size_t -> n:size_t{start + n <= len} -> lseq a n
-
-val slice: #a:Type -> #len:size_t -> lseq a len -> start:size_t -> fin:size_t{start <= fin /\ fin <= len} -> lseq a (fin - start)
-
-val update_sub: #a:Type -> #len:size_t -> lseq a len -> start:size_t -> n:size_t{start + n <= len} -> lseq a n -> lseq a len
-
-val update_slice: #a:Type -> #len:size_t -> lseq a len -> start:size_t -> fin:size_t{start <= fin /\ fin <= len} -> lseq a (fin - start) -> lseq a len
 
 type intseq (t:inttype) (len:size_t) = lseq (uint_t t) len
+type lbytes (len:size_t) = intseq U8 len
 
 val nat_from_intseq_be:#t:inttype -> #len:size_t -> b:intseq t len -> Tot (n:nat{n < pow2 (len `op_Multiply` bits t)})
 val nat_from_intseq_le:#t:inttype -> #len:size_t -> b:intseq t len -> Tot (n:nat{n < pow2 (len `op_Multiply` bits t)})
+
+val nat_from_bytes_be:#len:size_t -> b:lbytes len -> Tot (n:nat{n < pow2 (len `op_Multiply` 8)})
+val nat_from_bytes_le:#len:size_t -> b:lbytes len -> Tot (n:nat{n < pow2 (len `op_Multiply` 8)})
+
 val nat_to_bytes_le:
   len:size_t -> n:nat{n < pow2 (8 `op_Multiply` len)} ->  Tot (b:intseq U8 len {n == nat_from_intseq_le #U8 #len b})
 
